Split ufc into ufc_b and ufc_ub

src/LJF4_Rules.v
@@ -6,63 +6,65 @@ Global Arguments upd_rel_ex  {R A} _ _ _ _.
 
 From LJF Require Import LJF_SharedLogic. 
 
-Inductive ufc : ctx -> o -> state -> Prop :=
-| ufc_L_f :
+Inductive ufc_ub : ctx -> o -> Prop :=
+| ufc_ub_R_box :
+  forall {C: ctx} {D: o},
+    bracketable D ->
+    ufc_b C D ->
+    ufc_ub C D
+| ufc_ub_R_AndN :
+  forall {C: ctx} {B1 B2: o},
+    ufc_ub C B1 ->
+    ufc_ub C B2 ->
+    ufc_ub C (AndN B1 B2)
+| ufc_ub_R_Impl :
+  forall {C : ctx} {B1 B2: o},
+    ufc_ub ((B1, one) :: C) B2 ->
+    ufc_ub C (Impl B1 B2)
+
+with ufc_b : ctx -> o -> Prop :=
+| ufc_b_L_f :
   forall {C: ctx} {N : o} {K : o},
     exh C ->
     has_entry C (N, omega) ->
     negative N ->
     lfc C N K ->
-    ufc C K Bracketed
-| ufc_R_f :
+    ufc_b C K
+| ufc_b_R_f :
   forall {C: ctx} {P: o},
     exh C ->
     positive P ->
     rfc C P ->
-    ufc C P Bracketed
-| ufc_L_box :
+    ufc_b C P
+| ufc_b_L_box :
   forall {C C1 : ctx} {B : o} {K : o},
     upd_rel_ex C (B, one) (B, omega) C1 ->
     permeable B ->
-    ufc C1 K Bracketed ->
-    ufc C K Bracketed
-| ufc_R_box :
-  forall {C: ctx} {D: o},
-    bracketable D ->
-    ufc C D Bracketed ->
-    ufc C D Unbracketed
-| ufc_L_AndP :
+    ufc_b C1 K ->
+    ufc_b C K
+| ufc_b_L_AndP :
   forall {C C1: ctx} {B1 B2 : o} {K: o},
     has_entry C ((AndP B1 B2), one) ->
     upd_rel_ex C ((AndP B1 B2), one) ((AndP B1 B2), zero) C1 ->
-    ufc ((B1, one) :: (B2, one) :: C1) K Bracketed ->
-    ufc C K Bracketed
-| ufc_R_AndN :
-  forall {C: ctx} {B1 B2: o},
-    ufc C B1 Unbracketed ->
-    ufc C B2 Unbracketed->
-    ufc C (AndN B1 B2) Unbracketed
-| ufc_L_Or :
+    ufc_b ((B1, one) :: (B2, one) :: C1) K ->
+    ufc_b C K
+| ufc_b_L_Or :
   forall {C C1: ctx} {B1 B2 : o}  {K: o},
     has_entry C ((Or B1 B2), one) ->
     upd_rel_ex C ((Or B1 B2), one) ((Or B1 B2), zero) C1 ->
-    ufc ((B1, one) :: C1) K Bracketed ->
-    ufc ((B2, one) :: C1) K Bracketed ->
-    ufc C K Bracketed
-| ufc_R_Impl :
-  forall {C : ctx} {B1 B2: o},
-    ufc ((B1, one) :: C) B2 Unbracketed ->
-    ufc C (Impl B1 B2) Unbracketed
-| ufc_L_True :
+    ufc_b ((B1, one) :: C1) K ->
+    ufc_b ((B2, one) :: C1) K ->
+    ufc_b C K
+| ufc_b_L_True :
   forall {C C1: ctx}  {K: o},
     has_entry C (True, one) ->
     upd_rel_ex C (True, one) (True, zero) C1 ->
-    ufc C1 K Bracketed ->
-    ufc C K Bracketed
-| ufc_L_False :
+    ufc_b C1 K ->
+    ufc_b C K
+| ufc_b_L_False :
   forall {C: ctx}  {K: o},
     has_entry C (False, one) ->
-    ufc C K Bracketed
+    ufc_b C K
 
 (* First o for focused assumption, second o for conclusion K *)
 with lfc : ctx -> o -> o -> Prop :=
@@ -70,7 +72,7 @@ with lfc : ctx -> o -> o -> Prop :=
   forall {C : ctx} {P : o}  {K : o},
     exh C ->
     positive P ->
-    ufc ((P, one) :: C) K Bracketed ->
+    ufc_b ((P, one) :: C) K ->
     lfc C P K
 | lfc_I_l :
   forall {C: ctx} {N : o},
@@ -100,7 +102,7 @@ with rfc : ctx -> o -> Prop :=
   forall {C: ctx} {N: o},
     exh C ->
     negative N ->
-    ufc C N Unbracketed ->
+    ufc_ub C N ->
     rfc C N
 | rfc_I_r :
   forall {C: ctx} {P: o},
