src/LJF4_Prover.v
@@ -161,12 +161,12 @@ Ltac  T_lfc path ::=
 This will allow us to go through a emptying phase of the linear context after*)
 Ltac T_ufc_bracket path ::=
   lazymatch goal with
-  | [|- ufc _ ?k Unbracketed] =>
+  | [|- ufc_ub _ ?k ] =>
     let k' := (eval hnf in k) in
     lazymatch k' with
-    | AndN _ _ => apply ufc_R_AndN ; [> T_ufc_bracket path | T_ufc_bracket path]
-    | Impl _ _ => apply ufc_R_Impl ; T_ufc_bracket path
-    | _ => apply ufc_R_box ; [> T_bracketable | T_ufc_empty path]
+    | AndN _ _ => apply ufc_ub_R_AndN ; [> T_ufc_bracket path | T_ufc_bracket path]
+    | Impl _ _ => apply ufc_ub_R_Impl ; T_ufc_bracket path
+    | _ => apply ufc_ub_R_box ; [> T_bracketable | T_ufc_empty path]
     end
   end
 .
@@ -187,19 +187,19 @@ Ltac T_ufc_empty_private context path :=
     let b' := (eval hnf in b) in
     lazymatch b' with
     (*Next linear assumption is True*)
-    | True => eapply ufc_L_True ; [> T_has_entry | T_upd_rel_ex | T_ufc_empty_private rest path]
+    | True => eapply ufc_b_L_True ; [> T_has_entry | T_upd_rel_ex | T_ufc_empty_private rest path]
 
     (*Next linear assumption is False, must solve the branch*)
-    | False => solve [eapply ufc_L_False ; T_has_entry]
+    | False => solve [eapply ufc_b_L_False ; T_has_entry]
 
     (*Next linear assumption is a positive conjunction, we add the new assumptions to the list of linear assumption to process*)
-    | AndP ?B1 ?B2 => eapply ufc_L_AndP ; [> T_has_entry | T_upd_rel_ex | T_ufc_empty_private ((B1, one) :: (B2, one) :: rest) path]
+    | AndP ?B1 ?B2 => eapply ufc_b_L_AndP ; [> T_has_entry | T_upd_rel_ex | T_ufc_empty_private ((B1, one) :: (B2, one) :: rest) path]
 
     (*Next linear assumption is a disjunction, we add the new assumptions to the list of linear assumption to process*)
-    | Or ?B1 ?B2 => eapply ufc_L_Or ; [> T_has_entry | T_upd_rel_ex | T_ufc_empty_private ((B1, one) :: rest) path | T_ufc_empty_private ((B2, one) :: rest) path]
+    | Or ?B1 ?B2 => eapply ufc_b_L_Or ; [> T_has_entry | T_upd_rel_ex | T_ufc_empty_private ((B1, one) :: rest) path | T_ufc_empty_private ((B2, one) :: rest) path]
 
-    (*Next linear assumption is a positive atom or a negative formula. We place it in the structural context using ufc_L_box*)
-    | _ => eapply ufc_L_box ; [> T_upd_rel_ex | T_permeable | T_ufc_empty_private rest path]
+    (*Next linear assumption is a positive atom or a negative formula. We place it in the structural context using ufc_ub_L_box*)
+    | _ => eapply ufc_b_L_box ; [> T_upd_rel_ex | T_permeable | T_ufc_empty_private rest path]
     end
 
   (*Next assumption in context is either strucutural or already used*)
@@ -213,18 +213,18 @@ Ltac T_ufc_empty_private context path :=
 (*T_ufc_empty pattern matches on the goal to find the initial input to T_ifc_empty*)
 Ltac T_ufc_empty path ::=
   lazymatch goal with
-  | [|- ufc ?c _ Bracketed] => T_ufc_empty_private c path
+  | [|- ufc_b ?c _] => T_ufc_empty_private c path
   end
 .
 
 (*T_ufc_decide_right tries right focusing on a bracketed ufc sequent with exhausted context, if it fails or we cannot, we left focus instead*)
 Ltac T_ufc_decide_right path ::=
   lazymatch goal with
-  | [|- ufc ?c ?k Bracketed] =>
+  | [|- ufc_b ?c ?k] =>
     let k' := (eval hnf in k) in
     (*If k is positive, we right focus*)
     (*If k is negative, or right focusing fails, we left focus*)
-    solve [T_is_positive k' ; apply ufc_R_f ; [> T_exh | T_positive | T_rfc path]] || T_ufc_decide_left path
+    solve [T_is_positive k' ; apply ufc_b_R_f ; [> T_exh | T_positive | T_rfc path]] || T_ufc_decide_left path
   end
 .
 
@@ -244,7 +244,7 @@ Ltac T_ufc_decide_left_private context path :=
     (*If b is positive, or left focusing on b fail, we go to next entry*)
     | (?b, omega) :: ?rest => let b' := (eval hnf in b) in
     let npath := constr:((context', b) :: path) in
-    solve [T_is_negative b' ; T_noloop context' b path; eapply (@ufc_L_f _ b' _) ; [> T_exh | T_has_entry | T_negative | T_lfc npath]] || T_ufc_decide_left_private rest path
+    solve [T_is_negative b' ; T_noloop context' b path; eapply (@ufc_b_L_f _ b' _) ; [> T_exh | T_has_entry | T_negative | T_lfc npath]] || T_ufc_decide_left_private rest path
 
     (*On removed entry, we go to next entry*)
     | (_, zero) :: ?rest => T_ufc_decide_left_private rest path
@@ -260,7 +260,7 @@ Ltac T_ufc_decide_left_private context path :=
 (*T_ufc_decide_left pattern matches on the goal to find initial input to T_ufc_decide_left_private*)
 Ltac T_ufc_decide_left path ::=
   lazymatch goal with
-  | [|- ufc ?c _ Bracketed] => T_ufc_decide_left_private c path
+  | [|- ufc_b ?c _] => T_ufc_decide_left_private c path
   end
 .
 
@@ -270,8 +270,8 @@ Ltac T_solve :=
   lazymatch goal with
   | [|- lfc _ _ _] => T_lfc path
   | [|- rfc _ _] => T_rfc path
-  | [|- ufc _ _ Unbracketed] => T_ufc_bracket path
-  | [|- ufc _ _ Bracketed] => T_ufc_empty path
+  | [|- ufc_ub _ _] => T_ufc_bracket path
+  | [|- ufc_b _ _] => T_ufc_empty path
   | _ => fail "T_solve: goal is not a LFJ sequent"
   end
 .
